src/Narcissus/BinLib/AlignedDecodeMonad.v
@@ -1,4 +1,4 @@
-Require Import
+vRequire Import
         Bedrock.Word
         Coq.omega.Omega
         Coq.NArith.NArith
